src/sequential/SeqLiftAux.v
@@ -45,6 +45,229 @@ Require Import Pred.
 Require Import SeqLiftStep.
 
 
+Lemma added_memory_sim_promise_unmatch
+      f0 f1 srctm flag_src flag_tgt vers prom_tgt prom_src0 prom_src1 loc
+      msgs
+      (MEM: sim_promises srctm flag_src flag_tgt f0 vers prom_src0 prom_tgt)
+      (WF: Mapping.wfs f0)
+      (VERS: versions_wf f0 vers)
+      (ADDED: added_memory loc msgs prom_src0 prom_src1)
+      (FLAG: flag_src loc = true)
+      (MSGCOMPLETE: forall to_tgt from_tgt msg_tgt
+                           (GETTGT: Memory.get loc to_tgt prom_tgt = Some (from_tgt, msg_tgt)),
+          exists to_src from_src msg_src,
+            (<<TO: sim_timestamp_exact f1 f1.(Mapping.ver) to_src to_tgt>>) /\
+            (<<MSG: sim_message_max true loc to_src f0 (vers loc to_tgt) msg_src msg_tgt>>) /\
+            (<<CLOSED: Mapping.closed f1 f1.(Mapping.ver) to_src>>) /\
+            (<<IN: List.In (from_src, to_src, msg_src) msgs>>))
+      (MSGSOUND: forall to_src from_src msg_src
+                        (IN: List.In (from_src, to_src, msg_src) msgs),
+          (exists to_tgt,
+              (<<TO: sim_timestamp_exact f1 f1.(Mapping.ver) to_src to_tgt>>) /\
+              ((exists from_tgt msg_tgt,
+                   (<<FROM: sim_timestamp_exact f1 f1.(Mapping.ver) from_src from_tgt>>) /\
+                   (<<GET: Memory.get loc to_tgt prom_tgt = Some (from_tgt, msg_tgt)>>)) \/
+               ((<<TS: Time.lt (srctm loc) to_src>>) /\ (<<RESERVE: msg_src <> Message.reserve>>) /\ (<<NONE: forall val released (MSG: msg_src = Message.concrete val (Some released)), False>>) /\ (<<GET: Memory.get loc to_tgt prom_tgt = None>>)))))
+      (MAPWF: Mapping.wf f1)
+      (MAPLE: Mapping.le (f0 loc) f1)
+  :
+  let f' := (fun loc' => if Loc.eq_dec loc' loc then f1 else f0 loc') in
+  (<<SIM: sim_promises
+            srctm
+            (fun loc' => if Loc.eq_dec loc' loc then false else flag_src loc')
+            (fun loc' => if Loc.eq_dec loc' loc then true else flag_tgt loc')
+            f'
+            vers prom_src1 prom_tgt>>)
+.
+Proof.
+  pose proof (mapping_latest_wf_loc (f0 loc)) as VERWF.
+  assert (MAPSLE: Mapping.les f0 (fun loc' => if Loc.eq_dec loc' loc then f1 else f0 loc')).
+  { ii. des_ifs. refl. }
+  assert (MAPSWF: Mapping.wfs (fun loc' => if Loc.eq_dec loc' loc then f1 else f0 loc')).
+  { ii. des_ifs. }
+  ii. inv ADDED. econs.
+  { i. des_ifs.
+    { replace (f' loc) with f1.
+      2:{ unfold f'. des_ifs. }
+      hexploit MSGCOMPLETE; eauto. i. des.
+      hexploit MSGSOUND; eauto. i. des.
+      { eapply sim_timestamp_exact_unique in TO; eauto; ss. clarify.
+        esplits; eauto. erewrite <- sim_message_max_mon_mapping; eauto.
+      }
+      { eapply sim_timestamp_exact_unique in TO; eauto; ss. clarify. }
+    }
+    { hexploit sim_promises_get; eauto. i. des.
+      replace (f' loc0) with (f0 loc0).
+      { esplits; eauto.
+        erewrite <- sim_message_max_mon_mapping; eauto.
+      }
+      { unfold f'. des_ifs. }
+    }
+  }
+  { i. des_ifs.
+    { replace (f' loc) with f1.
+      2:{ unfold f'. des_ifs. }
+      hexploit SOUND; eauto. i. des.
+      { exfalso. hexploit sim_promises_none; eauto. rewrite GET0. ss. }
+      { hexploit MSGSOUND; eauto. i. des.
+        { left. esplits; eauto. }
+        { right. esplits; eauto. }
+      }
+    }
+    { replace (f' loc0) with (f0 loc0).
+      2:{ unfold f'. des_ifs. }
+      rewrite OTHER in GET; eauto.
+      hexploit sim_promises_get_if; eauto. i. des.
+      { left. esplits; eauto. }
+      { right. esplits; eauto. }
+    }
+  }
+  { i. des_ifs. rewrite OTHER; auto. eapply sim_promises_none; eauto. }
+Qed.
+
+
+Lemma mapped_msgs_exists f0 f1 vers srctm flag_src flag_tgt msgs_tgt prom_src prom_tgt loc
+      (PROM: sim_promises srctm flag_src flag_tgt f0 vers prom_src prom_tgt)
+      (MAPLE: Mapping.les f0 f1)
+      (MSGS: forall from to msg (IN: List.In (from, to, msg) msgs_tgt), Memory.get loc to prom_tgt = Some (from, msg))
+      (WF1: Mapping.wfs f1)
+  :
+    exists msgs_src,
+      (<<FORALL: List.Forall2
+                   (fun '(from_src, to_src, msg_src) '(from_tgt, to_tgt, msg_tgt) =>
+                      (<<FROM: sim_timestamp_exact (f1 loc) (f1 loc).(Mapping.ver) from_src from_tgt>>) /\
+                      (<<TO: sim_timestamp_exact (f1 loc) (f1 loc).(Mapping.ver) to_src to_tgt>>) /\
+                      (<<MESSAGE: sim_message_max (flag_tgt loc) loc to_src f1 (vers loc to_tgt) msg_src msg_tgt>>))
+                   msgs_src msgs_tgt>>).
+Proof.
+  revert MSGS. induction msgs_tgt; i.
+  { exists []. red. econs. }
+  destruct a as [[from_tgt to_tgt] msg_tgt].
+  hexploit MSGS.
+  { left. eauto. }
+  intros GETTGT. hexploit sim_promises_get; eauto.
+
+
+wf_cell_msgs
+
+
+(*   exists l : list (Time.t * Time.t * Message.t), *)
+(*     << *)
+(*     forall (from to : Time.t) (msg : Message.t), *)
+(*     << Cell.get to c = Some (from, msg) >> <-> << List.In (from, to, msg) l >> >> /\ *)
+(*     << wf_cell_msgs l >> *)
+
+
+(* wf_cell_msgs *)
+
+
+(*       (msgs: list (Time.t * Time.t * Message.t)) *)
+
+(*       sim_message_max_exists *)
+
+(*       wf_cell_msgs *)
+
+
+Lemma sim_thread_deflag_match_aux2
+      f0 vers flag_src flag_tgt vs_src vs_tgt
+      mem_src0 mem_tgt lc_src0 lc_tgt sc_src sc_tgt
+      loc
+      (SIM: sim_thread
+              f0 vers flag_src flag_tgt vs_src vs_tgt
+              mem_src0 mem_tgt lc_src0 lc_tgt sc_src sc_tgt)
+      (CONSISTENT: Local.promise_consistent lc_tgt)
+      (LOCALSRC: Local.wf lc_src0 mem_src0)
+      (LOCALTGT: Local.wf lc_tgt mem_tgt)
+      (MEMSRC: Memory.closed mem_src0)
+      (MEMTGT: Memory.closed mem_tgt)
+      (SCSRC: Memory.closed_timemap sc_src mem_src0)
+      (SCTGT: Memory.closed_timemap sc_tgt mem_tgt)
+      (WF: Mapping.wfs f0)
+      (FLAG: flag_src loc = true)
+      (VAL: option_rel Const.le (vs_tgt loc) (vs_src loc))
+      lang st
+  :
+    exists lc_src1 mem_src1 f1,
+      (<<STEPS: rtc (tau (@pred_step is_promise _))
+                    (Thread.mk lang st lc_src0 sc_src mem_src0)
+                    (Thread.mk _ st lc_src1 sc_src mem_src1)>>) /\
+      (<<SIM: sim_thread
+                f1 vers
+                (fun loc0 => if Loc.eq_dec loc0 loc then false else flag_src loc0)
+                (fun loc0 => if Loc.eq_dec loc0 loc then false else flag_tgt loc0)
+                vs_src vs_tgt
+                mem_src1 mem_tgt lc_src1 lc_tgt sc_src sc_tgt>>) /\
+      (<<WF: Mapping.wfs f1>>) /\
+      (<<MAPLE: Mapping.les f0 f1>>) /\
+      (<<UNCH: forall loc0 (NEQ: loc0 <> loc), f1 loc0 = f0 loc0>>) /\
+      (<<MAPFUTURE: map_future_memory f0 f1 mem_src1>>) /\
+      (<<SPACE: space_future_memory (unchangable mem_tgt lc_tgt.(Local.promises)) f0 mem_src0 f1 mem_src1>>)
+.
+Proof.
+  inv SIM. hexploit (MAXSRC loc). intros MAXTSSRC.
+  hexploit (MAXTGT loc). intros MAXTSTGT.
+  destruct (vs_src loc) eqn:VSRC; cycle 1.
+  { hexploit max_value_src_flag_none; eauto. i. clarify. }
+  inv MAXTSSRC. hexploit MAX; eauto. i. des.
+  destruct (vs_tgt loc) eqn:VTGT; ss.
+  inv MAXTSTGT. hexploit MAX1; eauto. i. des.
+  assert (TS: srctm loc = View.rlx (TView.cur tvw) loc).
+  { inv LOCAL. auto. }
+  hexploit sim_memory_top; eauto. intros TOP.
+  hexploit (@shifted_mapping_exists (f0 loc) (srctm loc)); eauto. i. des.
+
+  hexploit
+
+
+  (MSGCOMPLETE: forall to_tgt from_tgt msg_tgt
+                       (RESERVE: msg_tgt <> Message.reserve)
+                       (GETTGT: Memory.get loc to_tgt mem_tgt = Some (from_tgt, msg_tgt))
+                       (TS: Time.lt ts_tgt to_tgt),
+      exists to_src from_src msg_src,
+        (<<TO: sim_timestamp_exact f1 f1.(Mapping.ver) to_src to_tgt>>) /\
+        (<<MSG: sim_message false loc f0 (vers loc to_tgt) msg_src msg_tgt>>) /\
+        (<<CLOSED: forall val released (MSG: msg_tgt = Message.concrete val released), Mapping.closed f1 f1.(Mapping.ver) to_src>>) /\
+        (<<IN: List.In (from_src, to_src, msg_src) msgs>>))
+    (MSGSOUND: forall to_src from_src msg_src
+                      (IN: List.In (from_src, to_src, msg_src) msgs),
+        exists to_tgt from_tgt msg_tgt,
+          (<<TO: sim_timestamp_exact f1 f1.(Mapping.ver) to_src to_tgt>>) /\
+          (<<FROM: sim_timestamp_exact f1 f1.(Mapping.ver) from_src from_tgt>>) /\
+          (<<GET: Memory.get loc to_tgt mem_tgt = Some (from_tgt, msg_tgt)>>))
+
+    (MSGCOMPLETE: forall to_tgt from_tgt msg_tgt
+                         (GETTGT: Memory.get loc to_tgt prom_tgt = Some (from_tgt, msg_tgt)),
+        exists to_src from_src msg_src,
+          (<<TO: sim_timestamp_exact f1 f1.(Mapping.ver) to_src to_tgt>>) /\
+          (<<MSG: sim_message_max false loc to_src f0 (vers loc to_tgt) msg_src msg_tgt>>) /\
+          (<<CLOSED: Mapping.closed f1 f1.(Mapping.ver) to_src>>) /\
+          (<<IN: List.In (from_src, to_src, msg_src) msgs>>))
+    (MSGSOUND: forall to_src from_src msg_src
+                      (IN: List.In (from_src, to_src, msg_src) msgs),
+        exists to_tgt from_tgt msg_tgt,
+          (<<TO: sim_timestamp_exact f1 f1.(Mapping.ver) to_src to_tgt>>) /\
+          (<<FROM: sim_timestamp_exact f1 f1.(Mapping.ver) from_src from_tgt>>) /\
+          (<<GET: Memory.get loc to_tgt prom_tgt = Some (from_tgt, msg_tgt)>>))
+
+    (CLOSEDIF: forall ts (CLOSED: Mapping.closed f1 f1.(Mapping.ver) ts),
+        (<<CLOSED: Mapping.closed (f0 loc) (f0 loc).(Mapping.ver) ts>>) \/
+        (exists from val released, (<<IN: List.In (from, ts, Message.concrete val released) msgs>>)))
+
+         (WFMSGS: wf_cell_msgs msgs)
+         (FORALL: List.Forall
+                    (fun '(from, to, msg) => (__guard__((<<MAX: Time.le (Memory.max_ts loc mem0) from>>) \/ (<<RESERVE: msg = Message.reserve>>) /\ (<<DISJOINT: forall to2 from2 msg2 (GET: Memory.get loc to2 mem0 = Some (from2, msg2)), Interval.disjoint (from, to) (from2, to2)>>))) /\ (<<TS: Time.lt from to>>) /\ (<<MSGTO: Memory.message_to msg loc to>>) /\ (<<WF: Message.wf msg>>) /\ (<<CLOSED: semi_closed_message msg mem0 loc to>>)) msgs),
+
+
+
+
+  wf_cell_msgs
+
+add_promises_latest
+
+
+Admitted.
+
+
 Lemma sim_thread_deflag_match_aux2
       f0 vers flag_src flag_tgt vs_src vs_tgt
       mem_src0 mem_tgt lc_src0 lc_tgt sc_src sc_tgt
